\section{Семинар 5}

\subsection{Золотые пределы}

\begin{enumerate}
\item 
    \begin{equation*}
        \frac{e^{x} - 1}{x} \to 1, x \to 0
    .\end{equation*}

\item
    \begin{equation*}
        \frac{(1 + bx)^2 - 1}{x} \to \alpha b, x \to 0
    .\end{equation*}

\item
    \begin{equation*}
        \frac{a^{x} - 1}{x} \to \ln(a) (a > 0), x -> 0
    .\end{equation*}

\item
    \begin{equation*}
        \left(1 + \frac{\alpha}{x}\right)^{x} \to e^{\alpha}, x \to 0
    .\end{equation*}
\end{enumerate}

\subsection{Дааааа}

\begin{enumerate}
\item 
    \begin{align*}
        \lim_{x \to 0} \left\{ \frac{1 - \cos(x)\cos(2x)}{1 - \cos(x)} 
        = \frac{1 - \cos(x)\cos(2x) - \cos(2x) + \cos(2x)}{1 - \cos(x)} 
        = \frac{\cos(2x) (1 - \cos x)}{1 - \cos(x)} + \frac{1 - \cos(2x)}{1 - \cos(x)} 
        \right.
        \\
        \left. = \cos(2x) + \frac{1 - \cos(2x)}{(2x)^2} \cdot (2x)^2 \cdot \frac{x^2}{1 - \cos(x)}\frac{1}{x}
        \right\}
        \to 1 + 4 = 5
    .\end{align*}

\item
    \begin{equation*}
        \lim_{x \to 0} \left\{ x \cdot \ctg(5x) = \frac{x}{\tg(5x)} = \frac{5x}{\tg(5x)}\frac{1}{5} \right\} \to \frac{1}{5}
    .\end{equation*}

\item
    \begin{align*}
        \lim_{x \to 0} 
        \frac{(1 - x)(1 - \sqrt{x})(1 - \sqrt[3]{x}) \dots (1 - \sqrt[n]{x})}{(1 - x)^{n}}
    .\end{align*}
    \begin{equation*}
        x = 1 + t
    .\end{equation*}
    \begin{align*}
        &\lim_{t \to 0} \frac{-t(1 - \sqrt{1 + t})(1 - \sqrt[3]{1 + t}) \dots (1 - \sqrt[n]{1 + t})}{(-t)^{n}} \\
        = &\lim_{t \to 0} \frac{\sqrt{1 + t} - 1}{t} \cdot \frac{\sqrt[3]{1 + t} - 1}{t} \cdot \dots \cdot \frac{\sqrt[n]{1 + t} - 1}{t} \\
        \to &\frac{1}{2} \cdot \frac{1}{3} \cdot \dots \cdot \frac{1}{n} = \frac{1}{n!}
    .\end{align*}

\item
    \begin{equation*}
        \lim_{x \to 0} \left\{
        \left(1 + 3x^{4}\right)^{\frac{1}{\sin(x)^4}}
        = \left(1 + 3x^{4}\right)^{\frac{1}{3x^4} \cdot \frac{3x^4}{(\sin x)^4}}
        \right\}
        \to e^{3 \cdot 1^4} = e^3
    .\end{equation*}

\item
    \begin{equation*}
        \lim_{x \to 0} \left\{
            \frac{e^{x^2} - \cos x}{\sin^2 x}
            = \frac{e^{x^2} - 1}{\sin^2 x} + \frac{1 + \cos x}{\sin^2 x}
            = \frac{e^{x^2} - 1}{x^2} \cdot \frac{x^2}{\sin^2 x} + \frac{1 - \cos x}{x^2} \cdot \frac{x^2}{\sin^2 x}
        \right\}
        \to 1 \cdot 1^{-2} + \frac{1}{2} \cdot 1^{-2} = \frac{3}{2}
    .\end{equation*}

\item
    $\alpha = \frac{1}{2}$
    \begin{equation*}
        \lim_{x \to 0} \left\{ 
            \cos(x^{\alpha})^{\frac{1}{x}}
            = \left(1 - 2\sin^2\left(\frac{x^{\alpha}}{2}\right)\right)^{\frac{1}{x}}
            = \left(1 - 2\sin^2\left(\frac{x^{\alpha}}{2}\right)\right)^{\frac{1}{-2\sin^2\left(\frac{x^{\alpha}}{2}\right)} \cdot \frac{-2\sin^2\left(\frac{x^{\alpha}}{2}\right)}{x}}
        \right\}
        \to e^{1 (-2) \cdot \frac{1}{4}} = e^{-\frac{1}{2}}
    .\end{equation*}

    \begin{equation*}
        \lim_{x \to 0} \left\{
            \frac{\sin^2\left(\frac{x^{\alpha}}{2}\right)}{x} = \left(\frac{\sin^2 \frac{x^{\alpha}}{2}}{\frac{x^{\alpha}}{2}}\right)^2 \cdot \frac{\left(\frac{x^{a}}{2}\right)^2}{x}
        \right\} \to 1 \cdot \frac{1}{4}
    .\end{equation*}

    \begin{equation*}
        \lim_{x \to 0} \frac{1}{4} x^{2\alpha - 1} = \begin{cases}
            0 & \alpha > \frac{1}{2} \\
            \frac{1}{4} & \alpha = \frac{1}{2} \\
            \neg \exists & a \in (0, \frac{1}{2})
        \end{cases}
    .\end{equation*}

\item
    \begin{equation*}
        \lim_{x \to 0} \left\{
            \frac{\sqrt{3} - \sqrt{3 + x}}{\sin(2x)} = \sqrt{3} \cdot \frac{1 - \sqrt{1 + \frac{x}{3}}}{\frac{x}{3}} \cdot \frac{2x}{\sin (2x)} \cdot \frac{\frac{x}{3}}{2x}
        \right\}
        = \sqrt{3} (-\frac{1}{2}) \cdot 1 \cdot \frac{1}{6} = -\frac{\sqrt{3}}{12}
    .\end{equation*}

\item
    \begin{equation*}
        \lim_{x \to 0} \left(\sin \frac{1}{x} + \cos \frac{1}{x}\right)^x
    .\end{equation*}
\end{enumerate}
